normal and neutral predicates added - it's done!

Reduction.v
@@ -1,6 +1,7 @@
 Add LoadPath ".".
 
 Require Import SysF.
+Require Import Metatheory.
 Require Import Relations.
 
 Inductive reduction : term -> term -> Prop :=
@@ -66,27 +67,27 @@ End examples.
  * Congruence for ~>* *
  **********************)
 
-Lemma many_steps_congruence_abs (t t' : term) :
+Theorem many_steps_congruence_abs (t t' : term) :
   t ~>* t' -> forall T, abs T t ~>* abs T t'.
   intros. induction H; steps.
 Qed.
 
-Lemma many_steps_congruence_abs_t (t t' : term) :
+Theorem many_steps_congruence_abs_t (t t' : term) :
   t ~>* t' -> forall k, abs_t k t ~>* abs_t k t'.
   intros. induction H; steps.
 Qed.
 
-Lemma many_steps_congruence_app_left (t t' : term) :
+Theorem many_steps_congruence_app_left (t t' : term) :
   t ~>* t' -> forall t1, app t t1 ~>* app t' t1.
   intros. induction H; steps.
 Qed.
 
-Lemma many_steps_congruence_app_right (t t' : term) :
+Theorem many_steps_congruence_app_right (t t' : term) :
   t ~>* t' -> forall t1, app t1 t ~>* app t1 t'.
   intros. induction H; steps.
 Qed.
 
-Lemma many_steps_congruence_app_t (t t' : term) :
+Theorem many_steps_congruence_app_t (t t' : term) :
   t ~>* t' -> forall T, app_t t T ~>* app_t t' T.
   intros. induction H; steps.
 Qed.
@@ -96,7 +97,148 @@ Qed.
  ********************************************)
 
 Inductive normal : term -> Prop :=
-| var_normal n : normal (var n)
-| abs_normal T t : normal t -> normal (abs T t)
-| abs_t_normal k t : normal t -> normal (abs_t k t)
+| normal_neutral t : neutral t -> normal t
+| normal_abs T t : normal t -> normal (abs T t)
+| normal_abs_t k t : normal t -> normal (abs_t k t) 
+
+with neutral : term -> Prop :=
+     | neutral_var n : neutral (var n)
+     | neutral_app t1 t2 : neutral t1 -> normal t2 -> neutral (app t1 t2)
+     | neutral_app_t t T : neutral t -> neutral (app_t t T)
 .
+
+Ltac neutralize :=
+  simpl;
+  (eauto
+     || match goal with
+          | |- neutral (var _) => (apply neutral_var)
+          | |- neutral (app_t _ _) => (apply neutral_app_t; neutralize)
+          | |- neutral (app _ _) => (apply neutral_app; [ neutralize | normalize ])
+        end)
+  with normalize :=
+  simpl;
+  (eauto 
+     || match goal with
+          | |- normal (abs _ _) => (apply normal_abs; normalize)
+          | |- normal (abs_t _ _) => (apply normal_abs_t; normalize)
+          | |- normal _ => (apply normal_neutral; neutralize)
+        end).
+
+(***********************************************************************
+ * Proofs of correctness and completeness for the previous definitions *
+ ***********************************************************************)
+
+Section correctness_and_completeness.
+  Lemma normality_neutrality_correctness (t : term) (H : normal t \/ neutral t) :
+    forall t', ~ (t ~> t').
+    induction t; intros; intro; inversion H0.
+    - apply IHt in H4. apply H4. destruct H; inversion H.
+      inversion H5. left. apply H6.
+    - case H; intro; rewrite <- H2 in *; inversion H4;
+      [ inversion H5; inversion H9 | inversion H7 ].
+    - apply IHt1 in H4. apply H4. destruct H; inversion H.
+      + inversion H5. right. apply H9.
+      + right. apply H7.
+    - apply IHt2 in H4. apply H4. destruct H; inversion H.
+      + inversion H5. left. apply H10.
+      + left. apply H8.
+    - apply IHt in H4. apply H4. destruct H; inversion H; [ inversion H5 | left; apply H6 ].
+    - destruct H; inversion H; rewrite <- H2 in *.
+      + inversion H4. inversion H7.
+      + inversion H5.
+    - apply IHt in H4. apply H4. destruct H; inversion H.
+      + inversion H5. right. apply H8.
+      + right. apply H6.
+  Qed.
+  
+  Lemma normality_correctness (t : term) (H : normal t) (t' : term) : ~ (t ~> t').
+    eauto using normality_neutrality_correctness.
+  Qed.
+  
+  (* Stuck terms are incorrect terms that can't be reduced further *)
+  Inductive stuck : term -> Prop :=
+  | stuck_app k t t' : stuck (app (abs_t k t) t')
+  | stuck_app_t T t T' : stuck (app_t (abs T t) T')
+                               
+  | stuck_congr_abs T t : stuck t -> stuck (abs T t)
+  | stuck_congr_abs_t k t : stuck t -> stuck (abs_t k t)
+                                             
+  | stuck_congr_app_l t1 t2 : stuck t1 -> stuck (app t1 t2)
+  | stuck_congr_app_r t1 t2 : stuck t2 -> stuck (app t1 t2)
+  | stuck_congr_app_t t T : stuck t -> stuck (app_t t T).
+  
+  Ltac make_stuck :=
+    simpl; (eauto 
+              || (apply stuck_app)
+              || (apply stuck_app_t)
+              || (apply stuck_congr_abs; make_stuck)
+              || (apply stuck_congr_abs_t; make_stuck)
+              || (apply stuck_congr_app_l; [ make_stuck .. ])
+              || (apply stuck_congr_app_r; [ make_stuck .. ])
+              || (apply stuck_congr_app_t; make_stuck)).
+  
+  Lemma normality_completeness (t : term) :
+    (forall t', ~(t ~> t')) -> normal t \/ stuck t.
+    induction t; intros.
+    - left. normalize.
+    - assert (normal t0 \/ stuck t0).
+      { apply IHt. intros. intro. apply (H _ (congr_abs _ _ _ H0)). }
+      destruct H0; [ left; normalize | right; make_stuck ].
+    - assert (normal t1 \/ stuck t1).
+      { apply IHt1. intros. intro. apply (H _ (congr_app_left _ _ _ H0)). }
+      assert (normal t2 \/ stuck t2).
+      { apply IHt2. intros. intro. apply (H _ (congr_app_right _ _ _ H1)). }
+      destruct H0, H1; try (right; make_stuck).
+      + destruct t1.
+        * left. normalize.
+        * exfalso. apply (H (subst t1 0 t2)). one_step.
+        * left. inversion H0. eapply neutral_app in H2. apply normal_neutral. eauto. auto.
+        * right. make_stuck.
+        * left. inversion H0. normalize.
+    - assert (normal t \/ stuck t).
+        apply IHt. intros. intro. apply (H (abs_t k t')). one_step.
+        destruct H0; [ left; normalize | right; make_stuck ].
+      - assert (normal t \/ stuck t).
+        { apply IHt. intros. intro. apply (H (app_t t' t0)). one_step. }
+        destruct H0; try (right; make_stuck).
+        + destruct t.
+          * left. normalize.
+          * right. make_stuck.
+          * left. inversion H0. normalize.
+          * exfalso. apply (H (subst_typ t 0 t0)). one_step.
+          * left. inversion H0. normalize.
+    Qed.
+End correctness_and_completeness.
+
+(*************************************
+ * Preservation by type substitution *
+ *************************************)
+
+Lemma normality_neutrality_preservation :
+  forall (t : term) (pos : nat) (T : typ),
+    (normal t -> normal (subst_typ t pos T))
+    /\ (neutral t -> neutral (subst_typ t pos T)).
+  induction t; intros; simpl; try auto || split; intro.
+  - apply normal_abs. apply IHt. inversion H. inversion H0. normalize.
+  - inversion H.
+  - inversion H. inversion H0. apply normal_neutral, neutral_app.
+    + apply IHt1. neutralize.
+    + apply IHt2. neutralize.
+  - inversion H. apply neutral_app.
+    + apply IHt1. neutralize.
+    + apply IHt2. neutralize.
+  - apply normal_abs_t. apply IHt. inversion H. inversion H0. normalize. 
+  - inversion H.
+  - inversion H. inversion H0. apply normal_neutral. apply neutral_app_t. apply IHt. neutralize.
+  - inversion H. apply neutral_app_t. apply IHt. neutralize.
+Qed.
+
+Theorem normality_is_preserved_by_type_substitution (t : term) (H : normal t) :
+  forall (pos : nat) (T : typ), normal (subst_typ t pos T).
+  intros. apply normality_neutrality_preservation. auto.
+Qed.
+
+Theorem neutrality_is_preserved_by_type_substitution (t : term) (H : neutral t) :
+  forall (pos : nat) (T : typ), neutral (subst_typ t pos T).
+  intros. apply normality_neutrality_preservation. auto.
+Qed.
